dfy_exprs/NativeTypes.dfy
@@ -1,6 +1,7 @@
 module NativeTypes {
     type uint1 = i: int | 0 <= i < 2
     type uint32 = i:int | 0 <= i < 0x100000000
+ 	type uint256 = i:int | 0 <= i < 0x10000000000000000000000000000000000000000000000000000000000000000
 
     newtype{:nativeType "byte"} bit = i:int | 0 <= i < 2
     newtype{:nativeType "int"} int32 = i:int | -0x80000000 <= i < 0x80000000
